Let the equation of the circle be
%
\begin{equation}
\brak{x-h}^2 + \brak{y-k}^2 = r^2
\end{equation}
%
Since the circle touches the $y$-axis, the radius of the circle is $\abs{h}$ and $k = 2$.  Thus, the equation of the circle can be
expressed as
%
\begin{equation}
\brak{x-h}^2 + \brak{y-2}^2 = h^2
\end{equation}
%
Since the circle passes through the points  $\brak{-2,4}$, substituting these in the above equation yields
%
\begin{align}
\brak{h+2}^2 + 4 &= h^2 \\
\Rightarrow h = -2
\end{align}
%
Thus, the equation of the circle is
%
\begin{equation}
\brak{x+2}^2 + \brak{y-2}^2 = 4
\end{equation}
%
