The given function can be simplified as
%
\begin{align}
f\left(x\right)&=\tan ^{ -1 }{ \sqrt { \frac { 1+\sin { (x) }  }{ 1-\sin { (x) }  }  }  } \\
&= \tan ^{ -1 } \sqrt { \frac { 2 \cos ^2 \brak{\frac{\pi}{4}-\frac{x}{2}}  }{ 2 \cos ^2 \brak{\frac{\pi}{4}-\frac{x}{2}} }  } \\
& = \tan ^{ -1 } \cot \brak{\frac{\pi}{4}-\frac{x}{2}} \\
& = \frac{\pi}{4}+\frac{x}{2}
\end{align}
%
The normal to $f(x)$ has the equation
%
\begin{equation}
y = -2x + c,
\end{equation}
%
where $c$ is a constant. If $x = \frac{\pi}{6}, f(x) = \frac{\pi}{3}$.  Substituting the coordinates $\brak{\frac{\pi}{6},\frac{\pi}{3}}$ in the equation for the normal, $c = \frac{2\pi}{3}$. 

