Since the function is differentiable at $x=1$,
\begin{align}
\label{four_one}
\lim _{ x\rightarrow { 1 }^{ - } }{ f^{ \prime  }\left( x \right)  }  &= \lim _{ x\rightarrow { 1 }^{ + } }{ f^{ \prime  }\left(x \right)  }
\end{align}
Also,
%
\begin{align}
\label{four_two}
 \lim _{ x\rightarrow { 1 }^{ - } }{ f^{ \prime  }\left( x \right)  } &=-1 \\ 
\lim _{ x\rightarrow { 1 }^{ + } }{ f^{ \prime  }\left(x \right)  } &= -\frac { 1 }{ \sqrt { 1-{ (x+b) }^{ 2 } }  } 
\end{align}
%
From \eqref{four_one} and \eqref{four_two},
\begin{align}
-\frac { 1 }{ \sqrt { 1-{ (x+b) }^{ 2 } }} &= -1 \Rightarrow 
b &=-x = -1
\end{align}
Since a differentiable function is also continuous, 
\begin{align}
\lim _{ x\rightarrow { 1 }^{ + } }{ \quad a+\cos ^{ -1 }{ (x+b) }  } &= \lim _{ x\rightarrow { 1 }^{ - } }{ (-x) }  \\
\Rightarrow a+\frac { \pi  }{ 2 } &=-1\\
\Rightarrow a &=-1-\frac { \pi  }{ 2 }
\end{align}
Then
\begin{align}
  c=\frac{a}{b}=1+\frac { \pi  }{ 2 } 
\end{align}

