Let $P$ and $Q$ be $\brak{4t ^{ 2 }+3, 8 t ^{ 3 }-1}$ and 
 $\brak{4{ { t }_{ 1 } }^{ 2 }+3, 8  {t _{ 1 }} ^ 3 -1}$  respectively.
 At P, 
 \begin{align}
 \frac { dy }{ dx } = \frac { \frac { dy }{ dt } }{ \frac { dx }{ dt } }=\frac{24t^2}{8t}= 3t .
 \end{align}
 Since the tangent at $P$ meets the curve at $Q$, the equation of the tangent can be expressed as
 %
 \begin{align}
 \brak{y - 8t_1^3 +1} = 3t\brak{x - 4t_1^2 - 3}
 \end{align}
 %
 which, upon substitution of coordinates of $P$ yields
%
 \begin{align}
 \brak{8t^3 - 8t_1^3 } &= 3t\brak{4t^2 - 4t_1^2 }
 \\
\Rightarrow 8\brak{t_1 - t}({ { t }_{ 1 } }^{ 2 } + { t }_{ 1 } t + t^2) &= 3t. 4\brak{{ t }_{ 1 }  -t} \brak{{ t }_{ 1 }  + t } \nonumber
\\ 
\Rightarrow 2({ { t }_{ 1 } }^{ 2 }+ { { t }_{ 1 } }t + t^2) &= 3t({ t }_{ 1 }  + t)
 \\ 
\Rightarrow  2{ { t }_{ 1 } }^{ 2 } - t{ { t }_{ 1 } } - t^2 &= 0
\\
\Rightarrow  ({ t }_{ 1 }  - t) (2{ t }_{ 1 }  + t) &= 0
\\
 \Rightarrow  { t }_{ 1 } &= -\frac { t }{ 2 }
 \end{align}
 %
Thus, $Q$ can now be expressed as  $\brak{t^{ 2 }+3, t ^ 3 -1}$.  To demonstrate the solution of this problem, letting $t = 1$, we obtain $P,Q$ as $\brak{7,7},\brak{4,-2}$ respectively and the equation of the tangent is
%
\begin{align}
y-7 = 3\brak{x - 7}
\end{align}
%

