The solution can be obtained through the following cases
\begin{enumerate}
\item $\left( x^{2}-5x+5 \right) = 1$. This yields the solution 
\begin{equation}
\left( x-1 \right)\left( x-4 \right) = 0 \Rightarrow x = 1,4.
\end{equation}
\item $\left( x^{2}-5x+5 \right) = -1, \left( x^{2}+4x-60 \right)$ even. The first condition yields
%
\begin{align}
\left( x^{2}-5x+6 \right) &= 0
\\
\left( x-3 \right)\left( x-2 \right) &= 0 \Rightarrow x = 3 , 2
\end{align}
Testing the solutions for the second condition,
\begin{equation}
x^2+4x-60
= 
\begin{cases}
-39 & x = 3
\\
-48 & x = 2
\end{cases}
\end{equation}
giving $x =2$ as the desired solution.
%
\item Making the power 0,
\begin{equation}
x^{2}+4x-60 = 0 \Rightarrow x = -10 , 6.
\end{equation}
\end{enumerate}
%
Hence the required solutions are $x=1,4,2,6,-10$ and the sum of these roots is 3.
 
