Since the above expression is quadratic, let 
%
\begin{align}
\label{four_one}
\brak{1 + \frac{a}{x} - \frac{4}{x^2}}^{2x} &= \sbrak{\brak{1+\frac{\alpha}{ x}}\brak{1-\frac{\beta}{ x}}}^{2x} \\
&=\sbrak{\brak{1+\frac{\alpha}{ x}}^{\frac{x}{\alpha}}}^{2\alpha}\sbrak{\brak{1-\frac{\beta}{ x}}^{\frac{\beta}{x}}}^{2\beta} 
\end{align}
\begin{align}
\label{four_two}
\Rightarrow \lim_{x \rightarrow 0}\sbrak{\brak{1+\frac{\alpha}{ x}}^{\frac{x}{\alpha}}}^{2\alpha}\sbrak{\brak{1-\frac{\beta}{ x}}^{\frac{\beta}{x}}}^{2\beta} = e^{2\brak{\alpha-\beta}}
\end{align}
%
Thus, from \eqref{prob_four}, \eqref{four_one} and \eqref{four_two}, we obtain
%
\begin{align}
a &= \alpha -\beta
\\
2\brak{\alpha - \beta} = 3 
\\
\Rightarrow a = \frac{3}{2}
\end{align}
%
