\begin{multline}
\sum_{r=1}^{15} r^2 \frac{\binom{15}{r}}{\binom{15}{r-1}}
	= \  \sum_{r=1}^{15} r^2 \  \frac{15!}{r!\ (15-r)!} 
	\\
	\times   \frac{(r-1)!\ (15-r+1)!}{15!}
\end{multline}
%
which can be expressed as
	\begin{align}
	\  \sum_{r=1}^{15} r^2 \  \frac{(r-1)!}{r!} \  \frac{(16-r)!}{(15-r)!} 
	&= \  \sum_{r=1}^{15} r^2 \  \frac{(16-r)}{r}\\
	&= \  \sum_{r=1}^{15} (16r-r^2) \\
	&= \  16 \sum_{r=1}^{15} r \  - \  \sum_{r=1}^{15} r^2 \nonumber
\end{align}
resulting in
\begin{align}	
	&\  16 \cbrak{\frac{r\ (r+1)}{2}} \  - \  \frac{r\ (r+1)\ (2r+1)}{6}\\
	&= \  \frac{(48r^2 + 48r) \  - \  (2r^3 + 3r^2 + r)}{6}\\
	&= \  \frac{-2r^3 + 45r^2 + 47r}{6}
\end{align}
	




